## Q4

Base Case:

A is propositional symbol, $p$. Then, $p^u = (S[p])^t$ by definition.

Inductive Step:

IH: If $B$ and $C$ are sub formulas of $A$, then $B^u = (S[B])^t$ and $C^u = (S[C])^t$

Case 1: $A = \neg B$

By definition of substitution, $S[\neg B] = \neg S[B]$. Then,
$$
(\neg B)^u = (\neg S[B])^t \\
\neg(B^u) = \neg(S[B]^t) \\
\neg(S[B]^t) = \neg(S[B]^t) \\
LHS = RHS
$$

Case 2: $A = B\star C$

We have $S[B\star C] = S[B]\star S[C]$. Then,
$$
(B\star C)^u = (S[B]\star S[C])^t \\
B^u\star C^u = (S[B]^t\star S[C]^t) \\
(S[B])^t\star (S[C])^t = RHS
$$

By structural induction, our property holds.
