# A3

## Q1

### a)

$$
\begin{aligned}
A,\neg A & \vdash B \\
\neg A & \vdash A\to B & (\text{inconsistency law})
\end{aligned}
$$

### b)

$$
\begin{aligned}
\neg A & \vdash \neg A & (\in) \\
\neg A, \neg C & \vdash \neg A & (+) \\
\neg A & \vdash \neg C\to\neg A & (\to + ) \\
(A\to B)\to A,\neg A & \vdash A & (\text{modus ponens}, C|-| B) \\
(A\to B)\to A,\neg A & \vdash A\to \neg(A\to(A\to A)) & (C|-|\neg(A\to(A\to A))) \\
(A\to B)\to A & \vdash \neg A\to\neg(A\to(A\to A)) & (\to +) \\
(A\to B)\to A & \vdash (A\to (A\to A))\to A & (\text{contrapositive}) \\
(A\to B)\to A & \vdash A & ((A\to (A\to A))\to A |-| A) \\
\empty & \vdash ((A\to B)\to A)\to A & (\to +)
\end{aligned}
$$

### c)

$$

$$
